adequacy

L_Core_Adequacy.v
@@ -7,82 +7,114 @@ Set Implicit Arguments.
 Require Import LibLN.
 
 Require Import 
-  STLC_Core_Definitions 
-  STLC_Core_Infrastructure
-  STLC_Core_Soundness.
+  L_Core_Definitions 
+  L_Core_Infrastructure
+  L_Core_Soundness.
 
 (***************************************************************************)
 (** * Definitions with the exists-fresh quantification *)
 
 (** Terms are locally-closed pre-terms *)
 
-Inductive eterm : trm -> Prop :=
-  | eterm_var : forall x,
-      eterm (trm_fvar x)
-  | eterm_abs : forall x t1,
-      x \notin fv t1 ->
-      eterm (t1 ^ x) ->
-      eterm (trm_abs t1)
-  | eterm_app : forall t1 t2,
-      eterm t1 -> 
-      eterm t2 -> 
-      eterm (trm_app t1 t2).
+Inductive eprf :  prf -> Prop :=
+  | eprf_var : forall x,
+      eprf (prf_fvar x)
+  | eprf_abs : forall x p,
+      x \notin fv_prf p ->
+      eprf (p +^+ x) ->
+      eprf (prf_abs p)
+  | eprf_mu : forall a c,
+      a \notin fv_clos c ->
+      eclos (c *^- a) -> 
+      eprf (prf_mu c )
+with econt :  cont -> Prop :=
+  | econt_var : forall x,
+      econt (co_fvar x)
+  | econt_stack : forall p e,
+      eprf p->
+      econt e ->
+      econt (co_stack p e)
+  | econt_mut : forall a c,
+      a \notin fv_clos c ->
+      eclos (c *^+ a) -> 
+      econt (co_mut c )
+with eclos : clos -> Prop :=
+     | eclos_cl : forall p e,
+                    eprf p -> econt e -> eclos (cl p e).
 
 (** Typing relation *)
 
-Reserved Notation "E |== t ~: T" (at level 69).
+Reserved Notation "E |== p :+ T" (at level 69).
+Reserved Notation "E |== e :- T" (at level 69).
+Reserved Notation "c ::* E" (at level 69).
 
-Inductive etyping : env -> trm -> typ -> Prop :=
-  | etyping_var : forall E x T,
+
+Inductive etyping_prf : env -> prf -> typ -> Prop :=
+  | etyping_prf_var : forall E a T,
       ok E ->
-      binds x T E ->
-      E |== (trm_fvar x) ~: T
-  | etyping_abs : forall x E U T t1,
-      x \notin dom E \u fv t1 ->
-      (E & x ~ U) |== (t1 ^ x) ~: T ->
-      E |== (trm_abs t1) ~: (typ_arrow U T)
-  | etyping_app : forall S T E t1 t2,
-      E |== t1 ~: (typ_arrow S T) -> 
-      E |== t2 ~: S ->
-      E |== (trm_app t1 t2) ~: T
-
-where "E |== t ~: T" := (etyping E t T).
+      binds a (pos T) E ->
+      E |== (prf_fvar a) :+ T
+  | etyping_abs : forall x E U T p,
+      x \notin dom E \u fv_prf p ->
+      (E & x ~ pos U) |== (p +^+ x) :+ T ->
+      E |== (prf_abs p) :+ (typ_arrow U T)
+  | etyping_mu : forall a E T c,
+      a \notin dom E \u fv_clos c ->
+      (c::* E & a ~ neg T) ->
+      E |== prf_mu c :+ T
+with etyping_cont : env -> cont -> typ -> Prop :=
+  | etyping_cont_var : forall E a T,
+      ok E ->
+      binds a (neg T) E ->
+      E |== (co_fvar a) :- (T)
+  | etyping_mut : forall a E T c,
+      a \notin dom E \u fv_clos c -> 
+      c*^+a :* (E & a ~ pos T) ->
+      E |== (co_mut c) :- T
+  | etyping_stack : forall  E U T q e,
+     (E |== q :+ T ) -> 
+     ( E |== e :- U ) ->
+      E |== (co_stack q e) :- (typ_arrow T U)
+with etyping_clos : env -> clos -> Prop :=
+     | etyping_closure : forall E T p e,
+        (E |== p :+ T -> E |== e :- T -> (cl p e) ::* E)
+where "E |== p :+ T" := (etyping_prf E p T)
+and "E |== e :- T" := (etyping_cont E e T)
+and "c ::* E" := (etyping_clos E c)         .
 
 (** Definition of values (only abstractions are values) *)
 
-Inductive evalue : trm -> Prop :=
-  | evalue_abs : forall t1, 
-      eterm (trm_abs t1) -> evalue (trm_abs t1).
+Inductive evalue : prf -> Prop :=
+  | evalue_abs : forall p, 
+      eprf (prf_abs p) -> evalue (prf_abs p).
 
 (** Reduction relation - one step in call-by-value *)
+Inductive ered : clos -> clos -> Prop :=
+  | ered_mut : forall p c,
+      econt (co_mut c) ->
+      evalue p ->
+      ered (cl p (co_mut c)) (c*^^+ p)
+  | ered_abs : forall p q e,
+      eprf (prf_abs p) -> eprf q ->
+      econt e ->
+      ered (cl (prf_abs p) (co_stack q e)) (cl q (co_mut (cl p e)))
+  | ered_mu : forall e c ,
+      eprf (prf_mu c) -> econt e ->
+      ered (cl (prf_mu c) e) (c *^^- e).
 
-Inductive ered : trm -> trm -> Prop :=
-  | ered_beta : forall t1 t2,
-      eterm (trm_abs t1) ->
-      evalue t2 ->
-      ered (trm_app (trm_abs t1) t2) (t1 ^^ t2)
-  | ered_app_1 : forall t1 t1' t2,
-      eterm t2 ->
-      ered t1 t1' ->
-      ered (trm_app t1 t2) (trm_app t1' t2)
-  | ered_app_2 : forall t1 t2 t2',
-      evalue t1 ->
-      ered t2 t2' ->
-      ered (trm_app t1 t2) (trm_app t1 t2').
-
-Notation "t -->> t'" := (ered t t') (at level 68).
+Notation "c -->> c'" := (ered c c') (at level 68).
 
 (** Goal is to prove preservation and progress *)
 
-Definition epreservation := forall E t t' T,
-  E |== t ~: T ->
-  t -->> t' ->
-  E |== t' ~: T.
+Definition epreservation := forall E c c',
+  c ::* E ->
+  c --> c' ->
+   c'::* E.
 
-Definition eprogress := forall t T, 
-  empty |== t ~: T ->
-     evalue t 
-  \/ exists t', t -->> t'.
+Definition eprogress := forall p T, 
+  empty |== p :+ T ->
+     evalue p 
+  \/ forall a, a\notin fv_prf p -> exists c', cl p (co_fvar a) -->> c'.
 
 
 
@@ -93,48 +125,246 @@ Definition eprogress := forall t T,
 (* ********************************************************************** *)
 (** ** Proving the renaming lemma for [term]. *)
 
-Lemma term_rename : forall x y t,
-  term (t ^ x) ->
-  x \notin fv t -> 
-  y \notin fv t -> 
-  term (t ^ y).
+Lemma proof_rename_prf : forall x y p,
+  proof (p +^+ x) ->
+  x \notin fv_prf p -> 
+  y \notin fv_prf p -> 
+  proof (p +^+ y).
 Proof.
   introv Wx Frx Fry.
   (* introduce a renaming *)
-  rewrite (@subst_intro x). 
+  rewrite (@subst_intro_prf_prf x). 
   (* apply substitution result *)
-  apply* subst_term.
+  SearchAbout ([ _ ~+> _ ]+ _ +^+ _).
+  Print subst_prf_prf.
+  apply* proof_subst_prf_prf.
   (* use the fact that x is fresh *)
   assumption.
   (* prove term (trm_fvar y) *)
-  apply* term_var.
+  apply proof_var.
 Qed.
+
+Lemma proof_rename_cont : forall x y p,
+  proof (p +^- x) ->
+  x \notin fv_prf p -> 
+  y \notin fv_prf p -> 
+  proof (p +^- y).
+Proof.
+  introv Wx Frx Fry.
+  (* introduce a renaming *)
+  rewrite (@subst_intro_prf_cont x). 
+  (* apply substitution result *)
+  apply* proof_subst_prf_cont.
+  (* use the fact that x is fresh *)
+  assumption.
+  (* prove term (trm_fvar y) *)
+  apply context_var.
+Qed.
+
+Lemma context_rename_cont : forall x y e,
+  context (e -^- x) ->
+  x \notin fv_cont e -> 
+  y \notin fv_cont e  -> 
+  context (e -^- y).
+Proof.
+  introv Wx Frx Fry.
+  (* introduce a renaming *)
+  rewrite (@subst_intro_cont_cont x). 
+  (* apply substitution result *)
+  apply* context_subst_cont_cont.
+  (* use the fact that x is fresh *)
+  assumption.
+  (* prove term (trm_fvar y) *)
+  apply context_var.
+Qed.
+
+Lemma context_rename_prf : forall x y e,
+  context (e -^+ x) ->
+  x \notin fv_cont e -> 
+  y \notin fv_cont e  -> 
+  context (e -^+ y).
+Proof.
+  introv Wx Frx Fry.
+  (* introduce a renaming *)
+  rewrite (@subst_intro_cont_prf x). 
+  (* apply substitution result *)
+  apply* context_subst_cont_prf.
+  (* use the fact that x is fresh *)
+  assumption.
+  (* prove term (trm_fvar y) *)
+  apply proof_var.
+Qed.
+
+
+Lemma closure_rename_cont : forall x y c,
+  closure (c *^- x) ->
+  x \notin fv_clos c -> 
+  y \notin fv_clos c  -> 
+  closure (c *^- y).
+Proof.
+  introv Wx Frx Fry.
+  (* introduce a renaming *)
+  rewrite (@subst_intro_clos_cont x). 
+  (* apply substitution result *)
+  apply* closure_subst_clos_cont.
+  (* use the fact that x is fresh *)
+  assumption.
+  (* prove term (trm_fvar y) *)
+  apply context_var.
+Qed.
+
+Lemma closure_rename_prf : forall x y c,
+  closure (c *^+ x) ->
+  x \notin fv_clos c -> 
+  y \notin fv_clos c  -> 
+  closure (c *^+ y).
+Proof.
+  introv Wx Frx Fry.
+  (* introduce a renaming *)
+  rewrite (@subst_intro_clos_prf x). 
+  (* apply substitution result *)
+  apply* closure_subst_clos_prf.
+  (* use the fact that x is fresh *)
+  assumption.
+  (* prove term (trm_fvar y) *)
+  apply proof_var.
+Qed.
+
 
 (* ********************************************************************** *)
 (** ** Proving the renaming lemma for [typing]. *)
 
-Lemma typing_rename : forall x y E t U T,
-  (E & x ~ U) |= (t ^ x) ~: T -> 
-  x \notin dom E \u fv t ->
-  y \notin dom E \u fv t -> 
-  (E & y ~ U) |= (t ^ y) ~: T.
+Lemma typing_prf_rename_prf : forall x y E p U T,
+  (E & x ~ pos U) |= (p +^+ x) :+ T -> 
+  x \notin dom E \u fv_prf p ->
+  y \notin dom E \u fv_prf p -> 
+  (E & y ~ pos U) |= (p +^+ y) :+ T.
 Proof.
   introv Typx Frx Fry.
   (* ensure x <> y, so as to be able to build (E & y ~ U & x ~ U) *)
   tests: (x = y). subst*.
   (* assert that E is ok *)
-  lets K: (proj1 (typing_regular Typx)). destruct (ok_concat_inv K).
+  lets K: (proj1 (typing_regular_prf Typx)). destruct (ok_concat_inv K).
   (* introduce substitution *)
-  rewrite~ (@subst_intro x).
+  rewrite~ (@subst_intro_prf_prf x).
   (* apply substitution lemma *)
-  apply_empty* typing_subst.
+  Check typing_subst_prf.
+  apply_empty* typing_prf_subst_prf.
   (* apply weakening lemma *)
-  lets P: (@typing_weaken (x ~ U) E (y ~ U)). 
+  lets P: (@typing_prf_weaken (x ~ pos U) E (y ~ pos U)). 
    simpls. apply* P.
-  (* prove (E & y ~ U |= trm_fvar y ~: U) *)
-  apply* typing_var.
+  (* prove (E & y ~ U |= prf_fvar y :+ U) *)
+  apply* typing_prf_var.
 Qed.
 
+Lemma typing_prf_rename_cont : forall x y E p U T,
+  (E & x ~ neg U) |= (p +^- x) :+ T -> 
+  x \notin dom E \u fv_prf p ->
+  y \notin dom E \u fv_prf p -> 
+  (E & y ~ neg U) |= (p +^- y) :+ T.
+Proof.
+  introv Typx Frx Fry.
+  (* ensure x <> y, so as to be able to build (E & y ~ U & x ~ U) *)
+  tests: (x = y). subst*.
+  (* assert that E is ok *)
+  lets K: (proj1 (typing_regular_prf Typx)). destruct (ok_concat_inv K).
+  (* introduce substitution *)
+  rewrite~ (@subst_intro_prf_cont x).
+  (* apply substitution lemma *)
+  apply_empty* typing_prf_subst_cont.
+  (* apply weakening lemma *)
+  lets P: (@typing_prf_weaken (x ~ neg U) E (y ~ neg U)). 
+   simpls. apply* P.
+  apply* typing_cont_var.
+Qed.
+
+
+Lemma typing_cont_rename_prf : forall x y E e U T,
+  (E & x ~ pos U) |= (e -^+ x) :- T -> 
+  x \notin dom E \u fv_cont e ->
+  y \notin dom E \u fv_cont e -> 
+  (E & y ~ pos U) |= (e -^+ y) :- T.
+Proof.
+  introv Typx Frx Fry.
+  (* ensure x <> y, so as to be able to build (E & y ~ U & x ~ U) *)
+  tests: (x = y). subst*.
+  (* assert that E is ok *)
+  lets K: (proj1 (typing_regular_cont Typx)). destruct (ok_concat_inv K).
+  (* introduce substitution *)
+  rewrite~ (@subst_intro_cont_prf x).
+  (* apply substitution lemma *)
+  apply_empty* typing_cont_subst_prf.
+  (* apply weakening lemma *)
+  lets P: (@typing_cont_weaken (x ~ pos U) E (y ~ pos U)). 
+   simpls. apply* P.
+  apply* typing_prf_var.
+Qed.
+
+
+Lemma typing_cont_rename_cont : forall x y E e U T,
+  (E & x ~ neg U) |= (e -^- x) :- T -> 
+  x \notin dom E \u fv_cont e ->
+  y \notin dom E \u fv_cont e -> 
+  (E & y ~ neg U) |= (e -^- y) :- T.
+Proof.
+  introv Typx Frx Fry.
+  (* ensure x <> y, so as to be able to build (E & y ~ U & x ~ U) *)
+  tests: (x = y). subst*.
+  (* assert that E is ok *)
+  lets K: (proj1 (typing_regular_cont Typx)). destruct (ok_concat_inv K).
+  (* introduce substitution *)
+  rewrite~ (@subst_intro_cont_cont x).
+  (* apply substitution lemma *)
+  apply_empty* typing_cont_subst_cont.
+  (* apply weakening lemma *)
+  lets P: (@typing_cont_weaken (x ~ neg U) E (y ~ neg U)). 
+   simpls. apply* P.
+  apply* typing_cont_var.
+Qed.
+
+
+Lemma typing_clos_rename_prf : forall x y E c U,
+  (c *^+ x) :* (E & x ~ pos U) -> 
+  x \notin dom E \u fv_clos c ->
+  y \notin dom E \u fv_clos c -> 
+  (c *^+ y) :* (E & y ~ pos U).
+Proof.
+  introv Typx Frx Fry.
+  (* ensure x <> y, so as to be able to build (E & y ~ U & x ~ U) *)
+  tests: (x = y). subst*.
+  (* assert that E is ok *)
+  lets K: (proj1 (typing_regular_clos Typx)). destruct (ok_concat_inv K).
+  (* introduce substitution *)
+  rewrite~ (@subst_intro_clos_prf x).
+  (* apply substitution lemma *)
+  apply_empty* typing_clos_subst_prf.
+  (* apply weakening lemma *)
+  lets P: (@typing_clos_weaken (x ~ pos U) E (y ~ pos U)). 
+   simpls. apply* P.
+  apply* typing_prf_var.
+Qed.
+
+
+Lemma typing_clos_rename_cont : forall x y E c U,
+  (c *^- x) :* (E & x ~ neg U) -> 
+  x \notin dom E \u fv_clos c ->
+  y \notin dom E \u fv_clos c -> 
+  (c *^- y) :* (E & y ~ neg U).
+Proof.
+  introv Typx Frx Fry.
+  (* ensure x <> y, so as to be able to build (E & y ~ U & x ~ U) *)
+  tests: (x = y). subst*.
+  (* assert that E is ok *)
+  lets K: (proj1 (typing_regular_clos Typx)). destruct (ok_concat_inv K).
+  (* introduce substitution *)
+  rewrite~ (@subst_intro_clos_cont x).
+  (* apply substitution lemma *)
+  apply_empty* typing_clos_subst_cont.
+  (* apply weakening lemma *)
+  lets P: (@typing_clos_weaken (x ~ neg U) E (y ~ neg U)). 
+   simpls. apply* P.
+  apply* typing_cont_var.
+Qed.
 
 (***************************************************************************)
 (** * Proofs of equivalence.  *)
@@ -143,13 +373,19 @@ Qed.
 (* ********************************************************************** *)
 (** ** Proving the equivalence of [term] and [eterm] *)
 
-Hint Constructors term eterm.
+Hint Constructors proof eprf.
 
-Lemma term_to_eterm : forall t,
-  term t -> eterm t.
+Fixpoint proof_to_eprf p (Hp: proof p) {struct Hp}:  eprf p
+with context_to_econt e (He:context e) {struct He}: econt e
+with closure_to_eclos c (Hc:  closure c) {struct Hc}: eclos c.
 Proof.
-  induction 1; eauto.
-  pick_fresh x. apply* (@eterm_abs x).
+  - induction Hp.
+    + apply eprf_var.
+    + pick_fresh x. apply* (@eprf_abs x).
+    + pick_fresh x. apply* (@eprf_mu x).
+
+      apply closure_to_eclos.
+      
 Qed.
 
 Lemma eterm_to_term : forall t,
